Proofs about a valid plan

Compilation.thy
@@ -460,7 +460,7 @@ definition prob_automaton::"(alpha, ('proposition, 'action) clock, 'time, ('prop
 end
 
 context temporal_plan
-begin
+begin             
 
 abbreviation "B" where "B \<equiv> happ_at plan_happ_seq"
 
@@ -484,26 +484,134 @@ definition partial_exec_model::"(('proposition, 'action) clock, 'time) cval \<Ri
 "partial_exec_model W E \<equiv> \<forall>m < M. (W (Running (act m)) = 1 \<longleftrightarrow> (act m) \<in> E) \<and> (W (Running (act m)) = 0 \<longleftrightarrow> (act m) \<notin> E)"
 
 definition exec_state_sequence::"('time \<times> 'action) set" where
-"exec_state_sequence \<equiv> {(t, a) |s t a. (s, at_start a) \<in> plan_happ_seq \<and> s < t 
+"exec_state_sequence \<equiv> {(t, a) |s t a. a \<in> actions \<and> (s, at_start a) \<in> plan_happ_seq \<and> s < t 
                   \<and> \<not>(\<exists>s'. (s', at_end a) \<in> plan_happ_seq \<and> s \<le> s' \<and> s' < t)}"
 
 definition exec_state_sequence'::"('time \<times> 'action) set" where
-"exec_state_sequence' \<equiv> {(t, a) |s t a. (s, at_start a) \<in> plan_happ_seq \<and> s \<le> t 
+"exec_state_sequence' \<equiv> {(t, a) |s t a. a \<in> actions \<and> (s, at_start a) \<in> plan_happ_seq \<and> s \<le> t 
                   \<and> \<not>(\<exists>s'. (s', at_end a) \<in> plan_happ_seq \<and> s \<le> s' \<and> s' \<le> t)}"
 
+abbreviation "ES t \<equiv> {a. (t, a) \<in> exec_state_sequence}"
+
+abbreviation "IES t \<equiv> {a. (t, a) \<in> exec_state_sequence'}"
+
+lemma inc_es_is_next_es:
+  assumes "finite_plan"
+      and "Suc l < length htpl"
+  shows "IES (time_index l) = ES (time_index (Suc l))"
+proof (rule equalityI; rule subsetI)
+  fix a
+  assume "a \<in> IES (time_index l)"
+  then obtain s where
+    s: "a \<in> actions \<and> (s, at_start a) \<in> plan_happ_seq \<and> s \<le> time_index l"
+    "\<not>(\<exists>s'. (s', at_end a) \<in> plan_happ_seq \<and> s \<le> s' \<and> s' \<le> time_index l)"
+    unfolding exec_state_sequence'_def by blast
+  from this(2) time_index_ord[rotated, OF assms(2)] no_actions_between_indexed_timepoints[OF assms]
+  have "\<not>(\<exists>s'. (s', at_end a) \<in> plan_happ_seq \<and> s \<le> s' \<and> s' < time_index (Suc l))"
+    using happ_at_def by fastforce
+  with time_index_ord[rotated, OF \<open>Suc l < length htpl\<close>] s(1)
+  show "a \<in> ES (time_index (Suc l))" using exec_state_sequence_def by force
+next
+  fix a
+  assume "a \<in> ES (time_index (Suc l))"
+  then obtain s where
+    s: "a \<in> actions"
+    "(s, at_start a) \<in> plan_happ_seq"  
+    "s < time_index (Suc l)"
+    "\<not>(\<exists>s'. (s', at_end a) \<in> plan_happ_seq \<and> s \<le> s' \<and> s' < time_index (Suc l))"
+    unfolding exec_state_sequence_def by blast
+  from this(2, 3) no_actions_between_indexed_timepoints[OF assms]
+  have "s \<le> time_index l" using happ_at_def by fastforce
+  moreover
+  have "\<not>(\<exists>s'. (s', at_end a) \<in> plan_happ_seq \<and> s \<le> s' \<and> s' \<le> time_index l)" 
+  proof (rule notI)
+    assume "\<exists>s'. (s', at_end a) \<in> plan_happ_seq \<and> s \<le> s' \<and> s' \<le> time_index l"
+    with time_index_ord assms(2)
+    have "\<exists>s'. (s', at_end a) \<in> plan_happ_seq \<and> s \<le> s' \<and> s' < time_index (Suc l)" by fastforce
+    with s(4)
+    show "False" by blast
+  qed
+  ultimately
+  show "a \<in> IES (time_index l)" using s(1,2) exec_state_sequence'_def by blast
+qed
+
+lemma last_ies_empty:
+  assumes pap: "plan_actions_in_problem"
+      and dnz: "durations_non_zero"
+      and fp:  "finite_plan"
+  shows "IES (time_index (length htpl - 1)) = {}" (is "IES ?te = {}")
+proof -
+  have "a \<notin> IES ?te" for a
+  proof (rule notI)
+    assume a: "a \<in> IES ?te"
+    then obtain s where
+      s: "a \<in> actions"
+      "(s, at_start a) \<in> plan_happ_seq" 
+      "s \<le> ?te"
+      "\<not>(\<exists>s'. (s', at_end a) \<in> plan_happ_seq \<and> s \<le> s' \<and> s' \<le> ?te)"
+      using exec_state_sequence'_def by blast
+    from this(2)[simplified plan_happ_seq_def]
+    consider "(s, at_start a) \<in> {(t, at_start a)|a t d. (a, t, d) \<in> ran \<pi>}" 
+      | "(s, at_start a) \<in>  {(t + d, at_end a) |a t d. (a, t, d) \<in> ran \<pi>}"
+      by blast
+    then
+    have "\<exists>d. (a, s, d) \<in> ran \<pi>"
+    proof cases
+      case 1
+      hence "\<exists>a' t d. (s, at_start a) = (t, at_start a') \<and> (a', t, d) \<in> ran \<pi>" by simp
+      with assms(1)[simplified plan_actions_in_problem_def]
+      show ?thesis by (metis Pair_inject at_start_inj inj_on_contraD s(1))
+    next
+      case 2
+      hence "\<exists>a' t d. (s, at_start a) = (t + d, at_end a') \<and> (a', t, d) \<in> ran \<pi>" by auto
+      with s(1) assms(1)[simplified plan_actions_in_problem_def] snaps_disj
+      have False by blast
+      thus ?thesis ..
+    qed
+    then obtain d where
+      d: "(a, s, d) \<in> ran \<pi>"
+      "(s + d, at_end a) \<in> plan_happ_seq" using plan_happ_seq_def by blast
+    with s(4) assms(2)[simplified durations_non_zero_def]
+    have "s + d > ?te" by fastforce
+    
+    have "t \<le> ?te" if "t \<in> set htpl" for t
+    proof -
+      from that[simplified time_index_bij_betw_list[simplified bij_betw_def, THEN conjunct2, symmetric]]
+      obtain n where
+        n: "n < length htpl \<and> time_index n = t" by blast
+      show "t \<le> ?te"
+      proof (cases "n < length htpl - 1")
+        case True
+        with n
+        show ?thesis using time_index_ord by fastforce
+      next
+        case False
+        hence "n = length htpl - 1" using n by linarith
+        thus ?thesis using n by blast
+      qed
+    qed
+    moreover
+    
+    from d(1) set_htpl_eq_htps[OF fp] htps_def
+    have "s + d \<in> set htpl" by blast
+    ultimately
+    show False using \<open>s + d > ?te\<close> by fastforce
+  qed
+  thus "IES ?te = {}" by blast
+qed
 
 subsubsection \<open>Execution time\<close>
-definition argmax::"('ty::linordered_ab_group_add \<Rightarrow> bool) \<Rightarrow> 'ty" where
-"argmax P \<equiv> if (\<exists>x. P x) then (Greatest P) else 0"
+definition max_or_zero::"('ty::linordered_ab_group_add \<Rightarrow> bool) \<Rightarrow> 'ty" where
+"max_or_zero P \<equiv> if (\<exists>x. P x) then (Greatest P) else 0"
 
 definition last_snap_exec::"'snap_action \<Rightarrow> 'time \<Rightarrow> 'time" where
-"last_snap_exec a t = argmax (\<lambda>t'. t' < t \<and> a \<in> B t')"
+"last_snap_exec a t = max_or_zero (\<lambda>t'. t' < t \<and> a \<in> B t')"
 
 definition exec_time::"'snap_action \<Rightarrow> 'time \<Rightarrow> 'time" where
 "exec_time a t = (let t' = last_snap_exec a t in t - t')"
 
 definition last_snap_exec'::"'snap_action \<Rightarrow> 'time \<Rightarrow> 'time" where
-"last_snap_exec' a t = argmax (\<lambda>t'. t' \<le> t \<and> a \<in> B t')"
+"last_snap_exec' a t = max_or_zero (\<lambda>t'. t' \<le> t \<and> a \<in> B t')"
 
 definition exec_time'::"'snap_action \<Rightarrow> 'time \<Rightarrow> 'time" where
 "exec_time' a t = (let t' = last_snap_exec' a t in t - t')"
@@ -528,17 +636,68 @@ proof -
   have "(\<exists>x<t. a \<in> B x) = (\<exists>x\<le>t. a \<in> B x)"
     using nless_le by auto
   with \<open>a \<notin> B t\<close> 1
-  have "argmax (\<lambda>t'. t' < t \<and> a \<in> B t') = argmax (\<lambda>t'. t' \<le> t \<and> a \<in> B t')"
-    unfolding argmax_def using 1 by argo
+  have "max_or_zero (\<lambda>t'. t' < t \<and> a \<in> B t') = max_or_zero (\<lambda>t'. t' \<le> t \<and> a \<in> B t')"
+    unfolding max_or_zero_def using 1 by argo
   thus "last_snap_exec' a t = last_snap_exec a t"
     using last_snap_exec_def last_snap_exec'_def by simp
 qed
 
 lemma a_in_b_last_now: "a \<in> B t \<Longrightarrow> last_snap_exec' a t = t"
   unfolding last_snap_exec'_def
-  argmax_def
+  max_or_zero_def
   by (auto intro: Greatest_equality)
 
+lemma subseq_last_snap_exec: "(Suc l) < length htpl \<Longrightarrow> last_snap_exec a (time_index (Suc l)) = last_snap_exec' a (time_index l)"
+proof -
+  assume a: "(Suc l) < length htpl"
+  
+  have "last_snap_exec a (time_index (Suc l)) = max_or_zero (\<lambda>t'. t' < (time_index (Suc l)) \<and> a \<in> B t')"
+    unfolding last_snap_exec_def ..
+
+  define t where 
+    "t = max_or_zero (\<lambda>t'. t' < (time_index (Suc l)) \<and> a \<in> B t')"    
+
+  define s where
+    "s = max_or_zero (\<lambda>t'. t' \<le> (time_index l) \<and> a \<in> B t')" 
+  
+  have cl: "length htpl = card htps" using htpl_def by fastforce
+  
+  have tl_ord: "time_index l < time_index (Suc l)" 
+    using time_index_ord a
+    by blast
+  
+  from t_def consider "\<exists>t'. t' < (time_index (Suc l)) \<and> a \<in> B t'" 
+    | "\<not>(\<exists>t'. t' < (time_index (Suc l)) \<and> a \<in> B t')" by auto
+  hence "t = s"
+  proof cases
+    case 1
+    then obtain t' where
+      t': "t' < time_index (Suc l)" 
+      "a \<in> B t'" by blast
+    from this(2)
+    have "t' \<in> set htpl" using a_in_B_iff_t_in_htps 
+      using finite_htps htpl_def by auto
+    
+    from no_actions_between_indexed_timepoints[OF a] t' s_def
+    have "s = max_or_zero (\<lambda>t'. t' < (time_index (Suc l)) \<and> a \<in> B t')"
+      by (meson linorder_not_le order_less_le_trans tl_ord)
+    hence "t = s" using last_snap_exec_def t_def by blast
+    thus?thesis by simp
+  next
+    case 2
+    hence "\<not> (\<exists>t' \<le> time_index l. a \<in> B t')" using tl_ord by force
+    with 2 t_def[simplified max_or_zero_def] s_def[simplified max_or_zero_def]
+    show ?thesis  by auto
+  qed
+  thus "last_snap_exec a (time_index (Suc l)) = last_snap_exec' a (time_index l)" 
+    using s_def t_def last_snap_exec_def last_snap_exec'_def by auto
+  qed
+
+lemma updated_exec_time_and_next: 
+  assumes "Suc l < length htpl"
+  shows "exec_time a (time_index (Suc l)) = (exec_time' a (time_index l)) + (time_index (Suc l) - time_index l)"
+  using subseq_last_snap_exec[OF assms] exec_time_def exec_time'_def 
+  by simp
 
 subsubsection \<open>Restricting snap action sets by an upper limit on the index\<close>
 
@@ -576,95 +735,28 @@ abbreviation B_lim::"'time \<Rightarrow> nat \<Rightarrow> 'snap_action set" whe
 definition partial_exec_time_update::"'snap_action \<Rightarrow> 'time \<Rightarrow> nat \<Rightarrow> 'time" where
 "partial_exec_time_update a t m \<equiv> if (a \<in> B_lim t m) then 0 else exec_time a t"
 
-lemma B_lim_M_eq_B: "B_lim t M = B t" 
+lemma B_lim_M_eq_B:
+  assumes "plan_actions_in_problem"
+  shows "B_lim t M = B t" 
 proof (rule limit_M_eq_orig)
   show "B t \<subseteq> snap_actions"
   proof (rule subsetI)
     fix x
     assume "x \<in> B t"
     then have "\<exists>a. (x = at_start a \<or> x = at_end a) \<and> a \<in> actions" 
-      unfolding happ_at_def plan_happ_seq_def using plan_actions_in_problem
+      unfolding happ_at_def plan_happ_seq_def using assms(1)[simplified plan_actions_in_problem_def]
       by blast
     then show "x \<in> snap_actions" unfolding snap_actions_def by blast
   qed
 qed
 
-lemma exec_time_full_upd_eq_exec_time': "partial_exec_time_update a t M = exec_time' a t"
+lemma exec_time_full_upd_eq_exec_time': 
+  assumes "plan_actions_in_problem"
+  shows "partial_exec_time_update a t M = exec_time' a t"
   using partial_exec_time_update_def exec_time_def exec_time'_def 
-    a_not_in_b_last_unchanged a_in_b_last_now B_lim_M_eq_B 
+    a_not_in_b_last_unchanged a_in_b_last_now B_lim_M_eq_B[OF assms(1)]
   by simp 
 
-lemma subseq_last_snap_exec: "(Suc l) < length htpl \<Longrightarrow> last_snap_exec a (time_index (Suc l)) = last_snap_exec' a (time_index l)"
-proof -
-  assume a: "(Suc l) < length htpl"
-  
-  have "last_snap_exec a (time_index (Suc l)) = argmax (\<lambda>t'. t' < (time_index (Suc l)) \<and> a \<in> B t')"
-    unfolding last_snap_exec_def ..
-
-  define t where 
-    "t = argmax (\<lambda>t'. t' < (time_index (Suc l)) \<and> a \<in> B t')"    
-
-  define s where
-    "s = argmax (\<lambda>t'. t' \<le> (time_index l) \<and> a \<in> B t')" 
-  
-  have cl: "length htpl = card htps" using htpl_def by fastforce
-  
-  have tl_ord: "time_index l < time_index (Suc l)" 
-    using time_index_ord a
-    by blast
-  
-  from t_def consider "\<exists>t'. t' < (time_index (Suc l)) \<and> a \<in> B t'" 
-    | "\<not>(\<exists>t'. t' < (time_index (Suc l)) \<and> a \<in> B t')" by auto
-  hence "t = s"
-  proof cases
-    case 1
-    then obtain t' where
-      t': "t' < time_index (Suc l)" 
-      "a \<in> B t'" by blast
-    from this(2)
-    have "t' \<in> set htpl" using a_in_B_iff_t_in_htps 
-      using finite_htps htpl_def by auto
-    
-    have "\<not> (\<exists>t'. (time_index l) < t' \<and> t' < (time_index (Suc l)) \<and> t' \<in> set htpl)"
-    proof (rule notI)
-      assume "\<exists>t'>time_index l. t' < time_index (Suc l) \<and> t' \<in> set htpl"
-      with time_index_bij_betw_list
-      obtain l' where
-        l': "l' < length htpl"
-        "time_index l < time_index l'"
-        "time_index l' < time_index (Suc l)"
-        by (metis in_set_conv_nth)
-      hence "l' < (Suc l)"
-        by (metis not_less_iff_gr_or_eq time_index_ord)
-      moreover
-      have "l < l'" using l'
-        by (metis Suc_lessD a linorder_neqE_nat order_less_asym' time_index_ord)
-      ultimately
-      show "False" by simp
-    qed
-    hence nothing_happens: "\<not> (\<exists>t'>time_index l. t' < time_index (Suc l) \<and> a \<in> B t')"
-      using a_in_B_iff_t_in_htps finite_htps htpl_def by auto
-  
-    from nothing_happens t' s_def
-    have "s = argmax (\<lambda>t'. t' < (time_index (Suc l)) \<and> a \<in> B t')"
-      by (meson linorder_not_le order_less_le_trans tl_ord)      
-    hence "t = s" using last_snap_exec_def t_def by blast
-    thus?thesis by simp
-  next
-    case 2
-    hence "\<not> (\<exists>t' \<le> time_index l. a \<in> B t')" using tl_ord by force
-    with 2 t_def[simplified argmax_def] s_def[simplified argmax_def]
-    show ?thesis  by auto
-  qed
-  thus "last_snap_exec a (time_index (Suc l)) = last_snap_exec' a (time_index l)" 
-    using s_def t_def last_snap_exec_def last_snap_exec'_def by auto
-  qed
-
-lemma updated_exec_time_and_next: 
-  assumes "Suc l < length htpl"
-  shows "exec_time a (time_index (Suc l)) = (exec_time' a (time_index l)) + (time_index (Suc l) - time_index l)"
-  using subseq_last_snap_exec[OF assms] exec_time_def exec_time'_def 
-  by simp
 
 definition "W\<^sub>0 \<equiv> \<lambda>c. 0"
 
